shift-reset/var.v
@@ -1,3 +1,6 @@
 From Stdlib Require Import String.
 
 Record var : Type := Var { var_car : string }.
+
+Definition var_eq_dec : forall (v1 v2 : var), {v1 = v2} + {v1 <> v2}.
+Proof. decide equality; auto using string_dec. Defined.
